src/Pyrosome/Tools/Resolution.v
@@ -4,10 +4,9 @@ Require Import Datatypes.String Lists.List.
 Import ListNotations.
 Open Scope string.
 Open Scope list.
-From Utils Require Import Utils.
+From Utils Require Import Utils GallinaHintDb Ltac.
 From Pyrosome Require Import Theory.Core Tools.AllConstructors
-  Compilers.Compilers Compilers.CompilerFacts
-  Elab.Elab Elab.ElabCompilers.
+  Compilers.Compilers Compilers.CompilerFacts.
 Import Core.Notations.
 (*TODO: repackage this in compilers*)
 Import CompilerDefs.Notations.
@@ -860,26 +859,33 @@ Section WithVar.
 
   
 End WithVar.
+
+Create HintDb wf_lang_db discriminated.
+Create HintDb preserving_db discriminated.
+
+(* TODO: consider allowing other types than strings?*)
+Definition cmp_entry {a : lang string} {b c d} pf :=
+  let entry_ty p :=
+    preserving_compiler_ext (tgt_Model:=core_model (fst (fst (fst p))))
+      (snd (fst (fst p))) (snd (fst p)) (snd p)
+  in
+  mkEntry (exist entry_ty (a,b,c,d) pf).
+
+(* TODO: consider allowing other types than strings?*)
+Definition lang_entry {a : lang string} {b} pf :=
+  mkEntry (exist (fun p =>  wf_lang_ext (fst p) (snd p)) (a,b) pf).
   
-Ltac prove_by_lang_db dbP :=
-  apply (lang_wf_in_db_correct _ _ (proj2_sig dbP));
-  vm_compute; exact I.
+Ltac prove_by_lang_db :=
+  let db := ltac2val:(Ltac1.of_constr (hint_db_list "wf_lang_db")) in
+  apply (lang_wf_in_db_correct _ _ (proj2_sig (db_append_lang_list (V:=string) db)));
+  flagged_exact I.
 
 
-Ltac prove_by_cmp_db dbP :=
-  apply (cmp_wf_in_db_correct _ _ _ _ (proj2_sig dbP));
-  vm_compute; exact I.
+Ltac prove_by_cmp_db :=
+  let db := ltac2val:(Ltac1.of_constr (hint_db_list "preserving_db")) in
+  apply (cmp_wf_in_db_correct _ _ _ _ (proj2_sig (db_append_cmp_list (V:=string) db)));
+  flagged_exact I.
 
-(*TODO: this doesn't work since if 2 files overwrite it, importing 1 will erase the other*)
-(* set up a default db 
-Ltac2 mutable lang_db () := constr:(empty_dbP (V:=string)).
-
-*)
-
-(*TODO: update coq minimum version to use ltac2val 
-Tactic Notation "by_lang_db" :=
-  ltac2:(ltac1:(x|- prove_by_lang_db x)
-                 (Ltac1.of_constr (lang_db ()))).
-Tactic Notation "by_lang_db" constr(db) := prove_by_lang_db db.
-*)
-
+(*TODO: get rid of this *)
+Require Pyrosome.Tools.Matches.
+Ltac Matches.prove_from_known_elabs ::= prove_by_lang_db.
