src/Utils/Ltac.v
@@ -1,0 +1,28 @@
+From Ltac2 Require Import Ltac2 Std Option.
+Set Default Proof Mode "Classic".
+
+(* Uses vm_compute if do_check is idtac and vm_cast_no_check if do_check is fail*)
+Ltac exact_check_if do_check v :=
+  tryif do_check then (vm_compute; exact v)
+  else vm_cast_no_check v.
+
+Goal (if true then True else False).
+  exact_check_if idtac I.
+  Undo.
+  exact_check_if fail I.
+Abort.
+
+Goal (if false then True else False).
+  Fail exact_check_if idtac I.
+  exact_check_if fail I.
+Abort.
+
+(* Used to locally set a flag for checking computations during proof development *)
+Ltac2 mutable do_check_computations := false.
+
+Ltac2 flagged_exact p :=
+  if do_check_computations then vm_compute; exact $p
+  else vm_cast_no_check p.
+
+Ltac flagged_exact :=
+  ltac2:(p |- flagged_exact (get (Ltac1.to_constr p))).
